edr-system-model.ttool/AVATAR_executablecode/generated_src/fstar_src/parseSpeed.fst
@@ -22,24 +22,21 @@ noeq type struct_error = {
   message: C.String.t;
 }
 
-noeq type fstar_int32_array = {
-    value: B.buffer I32.t;
+noeq type fstar_uint8_array = {
+    value: B.buffer U8.t;
     error: struct_error;
 }
 
-// int32[] parseSpeed(uint32 can_id, uint8 can_dlc, uint8[] data)
 val parseSpeed_body:
   can_id: U32.t ->
   can_dlc: U8.t ->
   data: B.buffer U8.t ->
   
-Stack (fstar_int32_array: fstar_int32_array) (requires fun h0 -> 
-    // len(data) == 8 &&  can_id == 0x1b4 && can_dlc == 5 && get(data, 1) >= 0xD0 && get(data, 2) == 0 && get(data, 3) == 0 && get(data, 4) == 0 && len(data) == 8 && can_id == 0x1b4 && can_dlc == 5 && get(data, 1) >= 0xD0 && get(data, 2) == 0 && get(data, 3) == 0 && get(data, 4) == 0
-    B.live h0 data /\ (((B.length data) = (8)) && (U32.eq can_id 0x1b4ul) && (U8.eq can_dlc 5uy) && (U8.gte (B.get h0 data 1) 0xD0uy) && (U8.eq (B.get h0 data 2) 0uy) && (U8.eq (B.get h0 data 3) 0uy) && (U8.eq (B.get h0 data 4) 0uy) && ((B.length data) = (8)) && (U32.eq can_id 0x1b4ul) && (U8.eq can_dlc 5uy) && (U8.gte (B.get h0 data 1) 0xD0uy) && (U8.eq (B.get h0 data 2) 0uy) && (U8.eq (B.get h0 data 3) 0uy) && (U8.eq (B.get h0 data 4) 0uy))
+Stack (fstar_uint8_array: fstar_uint8_array) (requires fun h0 -> 
+    B.live h0 data /\ (((B.length data) = (8)) && (U32.eq can_id 0x1b4ul) && (U8.eq can_dlc 5uy) && (U8.gte (B.get h0 data 1) 0xD0uy) && (U8.eq (B.get h0 data 2) 0uy) && (U8.eq (B.get h0 data 3) 0uy) && (U8.eq (B.get h0 data 4) 0uy))
   )
-  (ensures fun h0 fstar_int32_array h1 -> 
-    // (fstar_int32_array.error.code == 0 && len(fstar_int32_array.value) == 2 ) || fstar_int32_array.error.code == 1
-    (((I32.eq fstar_int32_array.error.code 0l) && ((B.length fstar_int32_array.value) = (2))) || (I32.eq fstar_int32_array.error.code 1l))
+  (ensures fun h0 fstar_uint8_array h1 -> 
+    (((I32.eq fstar_uint8_array.error.code 0l) && ((B.length fstar_uint8_array.value) = (2))) || (I32.eq fstar_uint8_array.error.code 1l))
   )
 let parseSpeed_body can_id can_dlc data  =
     // TODO: you need to implement this function here
@@ -49,17 +46,15 @@ val parseSpeed:
   can_dlc: U8.t ->
   data: B.buffer U8.t ->
   
-  Stack (fstar_int32_array: fstar_int32_array) (requires fun h0 -> 
-    // len(data) == 8 &&  can_id == 0x1b4 && can_dlc == 5 && get(data, 1) >= 0xD0 && get(data, 2) == 0 && get(data, 3) == 0 && get(data, 4) == 0 && len(data) == 8 && can_id == 0x1b4 && can_dlc == 5 && get(data, 1) >= 0xD0 && get(data, 2) == 0 && get(data, 3) == 0 && get(data, 4) == 0
-    B.live h0 data /\ (((B.length data) = (8)) && (U32.eq can_id 0x1b4ul) && (U8.eq can_dlc 5uy) && (U8.gte (B.get h0 data 1) 0xD0uy) && (U8.eq (B.get h0 data 2) 0uy) && (U8.eq (B.get h0 data 3) 0uy) && (U8.eq (B.get h0 data 4) 0uy) && ((B.length data) = (8)) && (U32.eq can_id 0x1b4ul) && (U8.eq can_dlc 5uy) && (U8.gte (B.get h0 data 1) 0xD0uy) && (U8.eq (B.get h0 data 2) 0uy) && (U8.eq (B.get h0 data 3) 0uy) && (U8.eq (B.get h0 data 4) 0uy))
+  Stack (fstar_uint8_array: fstar_uint8_array) (requires fun h0 -> 
+    B.live h0 data /\ (((B.length data) = (8)))
   )
-  (ensures fun h0 fstar_int32_array h1 -> 
-    // (fstar_int32_array.error.code == 0 && len(fstar_int32_array.value) == 2 ) || fstar_int32_array.error.code == 1
-    (((I32.eq fstar_int32_array.error.code 0l) && ((B.length fstar_int32_array.value) = (2))) || (I32.eq fstar_int32_array.error.code 1l))
+  (ensures fun h0 fstar_uint8_array h1 -> 
+    (((I32.eq fstar_uint8_array.error.code 0l) && ((B.length fstar_uint8_array.value) = (2))) || (I32.eq fstar_uint8_array.error.code 1l))
   )
 let parseSpeed can_id can_dlc data  = 
     // meet the preconditions
-    if (let v1 = data.(1ul) in let v2 = data.(2ul) in let v3 = data.(3ul) in let v4 = data.(4ul) in let v5 = data.(1ul) in let v6 = data.(2ul) in let v7 = data.(3ul) in let v8 = data.(4ul) in ((U32.eq can_id 0x1b4ul) && (U8.eq can_dlc 5uy) && (U8.gte v1 0xD0uy) && (U8.eq v2 0uy) && (U8.eq v3 0uy) && (U8.eq v4 0uy) && (U32.eq can_id 0x1b4ul) && (U8.eq can_dlc 5uy) && (U8.gte v5 0xD0uy) && (U8.eq v6 0uy) && (U8.eq v7 0uy) && (U8.eq v8 0uy))) then
+    if (let v1 = data.(1ul) in let v2 = data.(2ul) in let v3 = data.(3ul) in let v4 = data.(4ul) in ((U32.eq can_id 0x1b4ul) && (U8.eq can_dlc 5uy) && (U8.gte v1 0xD0uy) && (U8.eq v2 0uy) && (U8.eq v3 0uy) && (U8.eq v4 0uy))) then
         parseSpeed_body can_id can_dlc data 
     else
         // TODO: you need to return an error value here if the preconditions are not met
